src/tools/parallelcomposition/parallelcompositionsimpleScript.sml
@@ -64,7 +64,7 @@ Define`
 *)
 
 (* multi transitions relation *)
-val _ = Parse.type_abbrev("mtrel", ``:(('symb set) # ('pred set) # 'state) -> ('event list) -> (('symb set) # ('pred set) # 'state)``);
+val _ = Parse.type_abbrev("mtrel", ``:(('symb set) # ('pred set) # 'state) -> ('event list) -> (('symb set) # ('pred set) # 'state) -> bool``);
 
 (* multi transitions system *)    
 val _ = Parse.type_abbrev("multransys", ``:(( 'symb, 'pred, 'state, 'event ) mtrel # ('pred) tded)``);
@@ -82,7 +82,24 @@ Define  `
         ((composeMuRe Re1 Re2 (Sym,P,S1,S2) [e] (Sym',P',S1',S2')) = (∃rel1 rel2. (composeRel rel1 rel2 (Sym,P,S1,S2) e (Sym',P',S1',S2')) ∧ (rel1 (Sym,(IMAGE OUTL P),S1) (OUTL e) (Sym',(IMAGE OUTL P'),S1')) ∧ (Re1 (Sym,(IMAGE OUTL P),S1) (MAP OUTL [e]) (Sym',(IMAGE OUTL P'),S1')) ∧ (rel2 (Sym,(IMAGE OUTR P),S2) (OUTR e) (Sym',(IMAGE OUTR P'),S2')) ∧ (Re2 (Sym,(IMAGE OUTR P),S2) (MAP OUTR [e]) (Sym',(IMAGE OUTR P'),S2'))))  ∧
 ((composeMuRe Re1 Re2 (Sym,P,S1,S2) (e::ev) (Sym'',P'',S1'',S2'')) = 
  (∃Sym' P' S1' S2' rel1 rel2 Re1' Re2'. (composeRel rel1 rel2 (Sym,P,S1,S2) e (Sym',P',S1',S2')) ∧ (rel1 (Sym,(IMAGE OUTL P),S1) (OUTL e) (Sym',(IMAGE OUTL P'),S1')) ∧ (Re1 (Sym,(IMAGE OUTL P),S1) (MAP OUTL (e::ev)) (Sym'',(IMAGE OUTL P''),S1'')) ∧ (rel2 (Sym,(IMAGE OUTR P),S2) (OUTR e) (Sym',(IMAGE OUTR P'),S2')) ∧ (Re2 (Sym,(IMAGE OUTR P),S2) (MAP OUTR (e::ev)) (Sym'',(IMAGE OUTR P''),S2'')) ∧ (Re2' (Sym',(IMAGE OUTR P'),S2') (MAP OUTR ev) (Sym'',(IMAGE OUTR P''),S2'')) ∧ (Re1' (Sym',(IMAGE OUTL P'),S1') (MAP OUTL ev) (Sym'',(IMAGE OUTL P''),S1'')) ∧ (composeMuRe Re1' Re2' (Sym',P',S1',S2') ev (Sym'',P'',S1'',S2''))))
-`;*)
+`;
+
+
+val composeMuRe_def =
+Define  `
+        ((composeMuRe (Re1:(('event1 + 'eventS), 'pred1, 'state1, 'symb) mtrel) (Re2:(('event2 + 'eventS), 'pred2, 'state2, 'symb) mtrel) (Sym,P,S1,S2) [] (Sym',P',S1',S2')) =
+         ((Sym,P,S1,S2) = (Sym',P',S1',S2')))  ∧
+((composeMuRe (Re1:(('event1 + 'eventS), 'pred1, 'state1, 'symb) mtrel) (Re2:(('event2 + 'eventS), 'pred2, 'state2, 'symb) mtrel) (Sym,P,S1,S2) [(INL (INL (E:'event1)))] (Sym',P',S1',S2')) =
+ ((Re1 (Sym,(IMAGE OUTL P),S1) [INL E] (Sym',(IMAGE OUTL P'),S1'))∧(S2 = S2')∧((IMAGE OUTR P) = (IMAGE OUTR P')))) ∧
+((composeMuRe (Re1:(('event1 + 'eventS), 'pred1, 'state1, 'symb) mtrel) (Re2:(('event2 + 'eventS), 'pred2, 'state2, 'symb) mtrel) (Sym,P,S1,S2) [(INR (INL (E:'event2)))] (Sym',P',S1',S2')) =
+ ((Re2 (Sym,(IMAGE OUTR P),S2) [INL E] (Sym',(IMAGE OUTR P'),S2'))∧(S1 = S1')∧((IMAGE OUTL P) = (IMAGE OUTL P')))) ∧
+((composeMuRe (Re1:(('event1 + 'eventS), 'pred1, 'state1, 'symb) mtrel) (Re2:(('event2 + 'eventS), 'pred2, 'state2, 'symb) mtrel) (Sym,P,S1,S2) [(INR (INR (E:'eventS)))] (Sym',P',S1',S2')) =
+ (∃Sym1' Sym2'. (Re1 (Sym,(IMAGE OUTL P),S1) [INR E] (Sym1',(IMAGE OUTL P'),S1'))∧(Re2 (Sym,(IMAGE OUTR P),S2) [INR E] (Sym2',(IMAGE OUTR P'),S2'))∧(Sym' = Sym1'∪Sym2'))) ∧
+((composeMuRe Re1 Re2 (Sym,P,S1,S2) (e::ev) (Sym'',P'',S1'',S2'')) = 
+ (∃Sym' P' S1' S2'. (composeMuRe Re1 Re2 (Sym,P,S1,S2) [e] (Sym',P',S1',S2')) ∧ (composeMuRe Re1 Re2 (Sym',P',S1',S2') ev (Sym'',P'',S1'',S2''))))
+`;  
+
+*)
 val FIRST_def =
 Define  `
         ((FIRST (a,b,c)) = a)
@@ -112,7 +129,7 @@ val triple_to_quadruple_thm = store_thm(
  FULL_SIMP_TAC std_ss [FIRST_def,SECOND_def,THIRD_def]  
   );
    
-(*        
+ (*       
 val composeMuRe_def =
 Define  `
         ((composeMuRe Re1 Re2 (Sym,P,S1,S2) [] (Sym',P',S1',S2')) = ((Sym,P,S1,S2) = (Sym',P',S1',S2')))  ∧
@@ -126,8 +143,21 @@ Define  `
                   (Re1 (Sym,(IMAGE OUTL P),S1) [INR E] (Sym1',(IMAGE OUTL P'),S1'))∧(Re2 (Sym,(IMAGE OUTR P),S2) [INR E] (Sym2',(IMAGE OUTR P'),S2'))∧(Sym' = Sym1'∪Sym2')))) ∧
         ((composeMuRe Re1 Re2 (Sym,P,S1,S2) (e::ev) (Sym'',P'',S1'',S2'')) = 
          (∃Sym' P' S1' S2'. (composeMuRe Re1 Re2 (Sym,P,S1,S2) [e] (Sym',P',S1',S2')) ∧ (composeMuRe Re1 Re2 (Sym',P',S1',S2') ev (Sym'',P'',S1'',S2''))))
-        `;
-*)
+        `;*)
+
+val composeMuRe_def =
+Define  `
+        ((composeMuRe (Re1:(('event1 + 'eventS), 'pred1, 'state1, 'symb) mtrel) (Re2:(('event2 + 'eventS), 'pred2, 'state2, 'symb) mtrel) (Sym,P,S1,S2) [] (Sym',P',S1',S2')) =
+         ((Sym,P,S1,S2) = (Sym',P',S1',S2')))  ∧
+((composeMuRe (Re1:(('event1 + 'eventS), 'pred1, 'state1, 'symb) mtrel) (Re2:(('event2 + 'eventS), 'pred2, 'state2, 'symb) mtrel) (Sym,P,S1,S2) ((INL (INL (E:'event1)))::ev) (Sym'',P'',S1'',S2'')) =
+ (∃Sym' P' S1'. (Re1 (Sym,(IMAGE OUTL P),S1) [INL E] (Sym',(IMAGE OUTL P'),S1'))∧((IMAGE OUTR P) = (IMAGE OUTR P'))∧ (composeMuRe Re1 Re2 (Sym',P',S1',S2) ev (Sym'',P'',S1'',S2'')))) ∧
+((composeMuRe (Re1:(('event1 + 'eventS), 'pred1, 'state1, 'symb) mtrel) (Re2:(('event2 + 'eventS), 'pred2, 'state2, 'symb) mtrel) (Sym,P,S1,S2) ((INR (INL (E:'event2)))::ev) (Sym'',P'',S1'',S2'')) =
+ (∃Sym' P' S2'. (Re2 (Sym,(IMAGE OUTR P),S2) [INL E] (Sym',(IMAGE OUTR P'),S2'))∧((IMAGE OUTL P) = (IMAGE OUTL P'))∧ (composeMuRe Re1 Re2 (Sym',P',S1,S2') ev (Sym'',P'',S1'',S2'')))) ∧
+((composeMuRe (Re1:(('event1 + 'eventS), 'pred1, 'state1, 'symb) mtrel) (Re2:(('event2 + 'eventS), 'pred2, 'state2, 'symb) mtrel) (Sym,P,S1,S2) ((INR (INR (E:'eventS)))::ev) (Sym'',P'',S1'',S2'')) =
+ (∃Sym1' Sym2' Sym' P' S1' S2'. (Re1 (Sym,(IMAGE OUTL P),S1) [INR E] (Sym1',(IMAGE OUTL P'),S1'))∧(Re2 (Sym,(IMAGE OUTR P),S2) [INR E] (Sym2',(IMAGE OUTR P'),S2'))∧(Sym' = Sym1'∪Sym2') ∧ (composeMuRe Re1 Re2 (Sym',P',S1',S2') ev (Sym'',P'',S1'',S2''))))
+`;                
+
+(*
 val composeMuRe_def =
 Define  `
         ((composeMuRe (Re1:(('event1 + 'eventS), 'pred1, 'state1, 'symb) mtrel) (Re2:(('event2 + 'eventS), 'pred2, 'state2, 'symb) mtrel) (Sym,P,S1,S2) []) = (Sym,P,S1,S2)) ∧
@@ -137,11 +167,11 @@ Define  `
  = composeMuRe Re1 Re2 ((FIRST(Re2 (Sym,(IMAGE OUTR P),S2) [INL E]),((IMAGE OUTL P)<+>(SECOND(Re2 (Sym,(IMAGE OUTR P),S2) [INL E]))),S1,THIRD(Re2 (Sym,(IMAGE OUTR P),S2) [INL E]))) ev) ∧
 ((composeMuRe (Re1:(('event1 + 'eventS), 'pred1, 'state1, 'symb) mtrel) (Re2:(('event2 + 'eventS), 'pred2, 'state2, 'symb) mtrel) (Sym,P,S1,S2) ((INR (INR (E:'eventS)))::ev))
  = composeMuRe Re1 Re2 (((FIRST(Re1 (Sym,(IMAGE OUTL P),S1) [INR E]))∪(FIRST(Re2 (Sym,(IMAGE OUTR P),S2) [INR E])),((SECOND(Re1 (Sym,(IMAGE OUTL P),S1) [INR E]))<+>(SECOND(Re2 (Sym,(IMAGE OUTR P),S2) [INR E]))),THIRD(Re1 (Sym,(IMAGE OUTL P),S1) [INR E]),THIRD(Re2 (Sym,(IMAGE OUTR P),S2) [INR E]))) ev)
-`;
+`;*)
 val composeMuRe_empty_event_thm = store_thm(
   "composeMuRe_empty_event_thm", ``
-∀Re1 Re2 Sym P S1 S2.
-(composeMuRe Re1 Re2 (Sym,P,S1,S2) []) = (Sym,P,S1,S2)
+∀Re1 Re2 Sym P S1 S2 Sym' P' S1' S2'.
+(composeMuRe Re1 Re2 (Sym,P,S1,S2) [] (Sym',P',S1',S2')) = ((Sym,P,S1,S2) = (Sym',P',S1',S2'))
                                        ``,
  FULL_SIMP_TAC std_ss [composeMuRe_def]  
   );
@@ -218,7 +248,7 @@ val (composeMuRe_rules, composeMuRe_ind, composeMuRe_cases)
    ((Evs = (e::ev)) ∧ (composeRel rel1 rel2 Conf e Conf') ∧ (Conf = (Sym,P,S1,S2)) ∧ (Conf' = (Sym',P',S1',S2')) ∧ (Conf'' = (Sym'',P'',S1'',S2'')) ∧ (rel1 (Sym,(IMAGE OUTL P),S1) (OUTL e) (Sym',(IMAGE OUTL P'),S1')) ∧ (Re1 (Sym,(IMAGE OUTL P),S1) (MAP OUTL Evs) (Sym'',(IMAGE OUTL P''),S1'')) ∧ (rel2 (Sym,(IMAGE OUTR P),S2) (OUTR e) (Sym',(IMAGE OUTR P'),S2')) ∧ (Re2 (Sym,(IMAGE OUTR P),S2) (MAP OUTR Evs) (Sym'',(IMAGE OUTR P''),S2'')) ∧ (Re2' (Sym',(IMAGE OUTR P'),S2') (MAP OUTR ev) (Sym'',(IMAGE OUTR P''),S2'')) ∧ (Re1' (Sym',(IMAGE OUTL P'),S1') (MAP OUTL ev) (Sym'',(IMAGE OUTL P''),S1'')) ∧ (composeMuRe Re1' Re2' Conf' ev Conf'')) ==> (composeMuRe Re1 Re2 Conf Evs Conf''))     
 `; 
 *)
-(* compose multi transition system *)(*
+(* compose multi transition system *)
 val _ = Parse.type_abbrev("MulComOpr", 
   ``:('symb, 'pred1, 'state1, 'event1 + 'eventS) multransys ->
   ('symb, 'pred2, 'state2, 'event2 + 'eventS) multransys -> 
@@ -234,13 +264,13 @@ val _ = set_mapped_fixity { fixity = Infixl 95,
                             tok = "||" };
 
 val _ = overload_on ("apply_composeMultiOperation", ``composeMultiOperation``);
-
+(*
  val composeMultiOperation_def =
 Define`
       (composeMultiOperation ((rel1:(('event1 + 'eventS), 'pred1, 'state1, 'symb) mtrel),(ded1:('pred1) tded)) ((rel2:(('event2 + 'eventS), 'pred2, 'state2, 'symb) mtrel),(ded2:('pred2) tded)) =
                              ((λ(Sym,P,S1,S2) E (Sym',P',S1',S2'). composeMuRe rel1 rel2 (Sym,P,S1,S2) E (Sym',P',S1',S2')), composeDed ded1 ded2): ('symb, 'pred1 + 'pred2, 'state1 # 'state2, (('event1+'eventS) + ('event2 +'eventS))) multransys)
-      `;*)
-
+      `;
+*)
 val combinelists_def =
 Define`
       (combinelists ([]:α list) ([]:β list) = (APPEND [] [])) ∧
@@ -248,10 +278,10 @@ Define`
 (combinelists ((e1::ev1):α list) ([]:β list) = APPEND (APPEND [INL e1] []) (combinelists ev1 [])) ∧
 (combinelists ((e1::ev1):α list) ((e2::ev2):β list) = APPEND (APPEND [INL e1] [INR e2]) (combinelists ev1 ev2))
 `;      
-
+(*
  val composeMultiOperation_def =
 Define`
       composeMultiOperation Re1 (Sym1,P1,S1) E1 Re2 (Sym2,P2,S2) E2 = (composeMuRe Re1 Re2 ((Sym1∪Sym2),(P1<+>P2),S1,S2) (combinelists E1 E2))
-      `;
+      `;*)
 val _ = export_theory();
 
